rocq-skylabs-brick/tests/source_location.v
@@ -9,6 +9,9 @@ Require Import skylabs.lang.cpp.syntax.mcore.
 Require Import skylabs.lang.cpp.parser.
 Require Import skylabs.lang.cpp.mparser.tu.
 Require Import skylabs.lang.cpp.parser.source_location.
+Require Import skylabs.prelude.parray.
+Require Import Stdlib.Numbers.Cyclic.Int63.Uint63.
+Require Import Stdlib.ZArith.ZArith.
 
 #[local] Notation lookup := syntax.source_location.lookup (only parsing).
 
@@ -48,7 +51,7 @@ Definition namespace_locations : declaration_locations origin_id := {|
 
 Definition namespace_map : source_map := {|
   files := [];
-  origins := test_origins;
+  origin_data := ExpandedOrigins test_origins;
   declarations := namespace_locations
 |}.
 
@@ -73,7 +76,7 @@ Definition nested_tree : loc_tree origin_id :=
 
 Definition nested_map : source_map := {|
   files := [];
-  origins := test_origins;
+  origin_data := ExpandedOrigins test_origins;
   declarations := {|
     symbol_locations := <[shared_root_name := nested_tree]> ∅;
     type_locations := ∅;
@@ -111,7 +114,7 @@ Proof. vm_compute. reflexivity. Qed.
 
 Definition invalid_id_map : source_map := {|
   files := [];
-  origins := test_origins;
+  origin_data := ExpandedOrigins test_origins;
   declarations := {|
     symbol_locations := <[shared_root_name := leaf [1; 9; 8]]> ∅;
     type_locations := ∅;
@@ -130,7 +133,7 @@ Definition invalid_anchor_origin : source_origin :=
 
 Definition invalid_anchor_map : source_map := {|
   files := [];
-  origins := [invalid_anchor_origin];
+  origin_data := ExpandedOrigins [invalid_anchor_origin];
   declarations := {|
     symbol_locations := <[shared_root_name := leaf [0]]> ∅;
     type_locations := ∅;
@@ -149,7 +152,7 @@ Definition invalid_derived_origin : source_origin :=
 
 Definition invalid_derived_map : source_map := {|
   files := [];
-  origins := [invalid_derived_origin];
+  origin_data := ExpandedOrigins [invalid_derived_origin];
   declarations := {|
     symbol_locations := <[shared_root_name := leaf [0]]> ∅;
     type_locations := ∅;
@@ -168,7 +171,7 @@ Definition valid_reference_origin : source_origin :=
 
 Definition valid_reference_map : source_map := {|
   files := [];
-  origins := [origin0; valid_reference_origin];
+  origin_data := ExpandedOrigins [origin0; valid_reference_origin];
   declarations := {|
     symbol_locations := <[shared_root_name := leaf [1]]> ∅;
     type_locations := ∅;
@@ -184,7 +187,7 @@ Proof. vm_compute. reflexivity. Qed.
 
 Definition ordered_multi_origin_map : source_map := {|
   files := [];
-  origins := test_origins;
+  origin_data := ExpandedOrigins test_origins;
   declarations := {|
     symbol_locations := <[shared_root_name := leaf [2; 0; 3; 1]]> ∅;
     type_locations := ∅;
@@ -198,10 +201,397 @@ Example lookup_preserves_explicit_multi_origin_order :
     inr [origin2; origin0; origin3; origin1].
 Proof. vm_compute. reflexivity. Qed.
 
+Definition indexed_table_of_list {A : Type}
+    (default : A) (values : list A) : Encoded.indexed_table A :=
+  Encoded.Build_indexed_table
+    (Uint63.of_Z (Z.of_nat (List.length values)))
+    (PArray.of_list (PArray.of_list default [])
+      [PArray.of_list default values]).
+
+Definition simple_encoded_origins : list Encoded.encoded_origin :=
+  [ Encoded.Build_encoded_origin ExplicitOrigin
+      None None None None [] None None []
+  ; Encoded.Build_encoded_origin ImplicitOrigin
+      None None None None [] None None []
+  ; Encoded.Build_encoded_origin ClangTransformedOrigin
+      None None None None [] None None []
+  ; Encoded.Build_encoded_origin Cpp2vSynthesizedOrigin
+      None None None None [] None None []
+  ].
+
+Definition simple_indexed_provenance : Encoded.indexed_provenance :=
+  Encoded.Build_indexed_provenance
+    (indexed_table_of_list Encoded.default_presumed_filename [])
+    (indexed_table_of_list Encoded.default_physical_point [])
+    (indexed_table_of_list Encoded.default_encoded_presumed_point [])
+    (indexed_table_of_list Encoded.default_encoded_range [])
+    (indexed_table_of_list Encoded.default_encoded_macro_frame [])
+    (indexed_table_of_list Encoded.default_encoded_origin
+      simple_encoded_origins).
+
+Definition indexed_namespace_map : source_map := {|
+  files := [];
+  origin_data := IndexedOrigins simple_indexed_provenance;
+  declarations := namespace_locations
+|}.
+
+Example indexed_lookup_symbol_namespace_parity :
+  lookup indexed_namespace_map (DRSymbol shared_root_name) [] =
+    lookup namespace_map (DRSymbol shared_root_name) [].
+Proof. vm_compute. reflexivity. Qed.
+
+Example indexed_lookup_type_namespace_parity :
+  lookup indexed_namespace_map (DRType shared_root_name) [] =
+    lookup namespace_map (DRType shared_root_name) [].
+Proof. vm_compute. reflexivity. Qed.
+
+Example indexed_lookup_template_namespaces_parity :
+  ( lookup indexed_namespace_map (DRMsymbol shared_root_name) []
+  , lookup indexed_namespace_map (DRMtype shared_root_name) [] ) =
+  ( lookup namespace_map (DRMsymbol shared_root_name) []
+  , lookup namespace_map (DRMtype shared_root_name) [] ).
+Proof. vm_compute. reflexivity. Qed.
+
+Definition indexed_nested_map : source_map := {|
+  files := [];
+  origin_data := IndexedOrigins simple_indexed_provenance;
+  declarations := nested_map.(declarations)
+|}.
+
+Example indexed_lookup_path_and_empty_parity :
+  ( lookup indexed_nested_map (DRSymbol shared_root_name) []
+  , lookup indexed_nested_map (DRSymbol shared_root_name) [0]
+  , lookup indexed_nested_map (DRSymbol shared_root_name) [1; 0]
+  , lookup indexed_nested_map (DRSymbol shared_root_name) [1] ) =
+  ( lookup nested_map (DRSymbol shared_root_name) []
+  , lookup nested_map (DRSymbol shared_root_name) [0]
+  , lookup nested_map (DRSymbol shared_root_name) [1; 0]
+  , lookup nested_map (DRSymbol shared_root_name) [1] ).
+Proof. vm_compute. reflexivity. Qed.
+
+Example indexed_lookup_root_and_child_error_parity :
+  ( lookup indexed_nested_map (DRSymbol absent_root_name) []
+  , lookup indexed_nested_map (DRSymbol shared_root_name) [2]
+  , lookup indexed_nested_map (DRSymbol shared_root_name) [1; 1] ) =
+  ( lookup nested_map (DRSymbol absent_root_name) []
+  , lookup nested_map (DRSymbol shared_root_name) [2]
+  , lookup nested_map (DRSymbol shared_root_name) [1; 1] ).
+Proof. vm_compute. reflexivity. Qed.
+
+Definition indexed_invalid_id_map : source_map := {|
+  files := [];
+  origin_data := IndexedOrigins simple_indexed_provenance;
+  declarations := invalid_id_map.(declarations)
+|}.
+
+Example indexed_lookup_invalid_origin_parity :
+  lookup indexed_invalid_id_map (DRSymbol shared_root_name) [] =
+    lookup invalid_id_map (DRSymbol shared_root_name) [].
+Proof. vm_compute. reflexivity. Qed.
+
+Definition indexed_ordered_map : source_map := {|
+  files := [];
+  origin_data := IndexedOrigins simple_indexed_provenance;
+  declarations := ordered_multi_origin_map.(declarations)
+|}.
+
+Example indexed_lookup_origin_order_parity :
+  lookup indexed_ordered_map (DRSymbol shared_root_name) [] =
+    lookup ordered_multi_origin_map (DRSymbol shared_root_name) [].
+Proof. vm_compute. reflexivity. Qed.
+
+Definition rich_points : list physical_point :=
+  [ Build_physical_point 0 1%N 2%N 3%N
+  ; Build_physical_point 0 4%N 5%N 6%N
+  ; Build_physical_point 0 7%N 8%N 9%N
+  ; Build_physical_point 0 10%N 11%N 12%N
+  ].
+
+Definition rich_ranges : list Encoded.encoded_range :=
+  [ Encoded.EncodedRawRange (Some 0%uint63) None CharacterRange
+  ; Encoded.EncodedSameBeginRange 0%uint63 1%uint63 TokenRange 1%uint63
+  ; Encoded.EncodedGeneralRange 0%uint63 1%uint63 CharacterRange
+      2%uint63 3%uint63
+  ].
+
+Definition rich_frame : Encoded.encoded_macro_frame :=
+  Encoded.Build_encoded_macro_frame (Some "MACRO"%pstring) MacroArgument
+    (Some 0%uint63) (Some 1%uint63).
+
+Definition rich_inline_frame : Encoded.encoded_macro_frame :=
+  Encoded.Build_encoded_macro_frame (Some "INLINE"%pstring) MacroBody
+    (Some 2%uint63) None.
+
+Definition rich_encoded_origin : Encoded.encoded_origin :=
+  Encoded.Build_encoded_origin ExplicitOrigin
+    (Some 2%uint63) (Some 1%uint63)
+    (Some 0%uint63) (Some 1%uint63)
+    [ Encoded.MacroFrameReference 0%uint63
+    ; Encoded.InlineMacroFrame rich_inline_frame
+    ] (Some 3%uint63) (Some 1) [1].
+
+Definition rich_reference_encoded_origin : Encoded.encoded_origin :=
+  Encoded.Build_encoded_origin ImplicitOrigin
+    None None None None [] None None [].
+
+Definition rich_indexed_provenance : Encoded.indexed_provenance :=
+  Encoded.Build_indexed_provenance
+    (indexed_table_of_list Encoded.default_presumed_filename
+      ["logical.cpp"%pstring])
+    (indexed_table_of_list Encoded.default_physical_point rich_points)
+    (indexed_table_of_list Encoded.default_encoded_presumed_point
+      [ Encoded.Build_encoded_presumed_point 0%uint63 20%N 21%N
+      ; Encoded.Build_encoded_presumed_point 0%uint63 22%N 23%N
+      ])
+    (indexed_table_of_list Encoded.default_encoded_range rich_ranges)
+    (indexed_table_of_list Encoded.default_encoded_macro_frame [rich_frame])
+    (indexed_table_of_list Encoded.default_encoded_origin
+      [rich_encoded_origin; rich_reference_encoded_origin]).
+
+Definition rich_origin : source_origin :=
+  Build_source_origin ExplicitOrigin
+    (Some (Build_source_range
+      (Some (Build_physical_point 0 1%N 2%N 3%N))
+      (Some (Build_physical_point 0 4%N 5%N 6%N)) CharacterRange
+      (Some (Build_physical_point 0 7%N 8%N 9%N,
+             Build_physical_point 0 10%N 11%N 12%N))))
+    (Some (Build_source_range
+      (Some (Build_physical_point 0 1%N 2%N 3%N))
+      (Some (Build_physical_point 0 4%N 5%N 6%N)) TokenRange
+      (Some (Build_physical_point 0 1%N 2%N 3%N,
+             Build_physical_point 0 4%N 5%N 6%N))))
+    (Some (Build_presumed_point "logical.cpp"%pstring 20%N 21%N))
+    (Some (Build_presumed_point "logical.cpp"%pstring 22%N 23%N))
+    [ Build_macro_frame (Some "MACRO"%pstring) MacroArgument
+        (Some (Build_source_range
+          (Some (Build_physical_point 0 1%N 2%N 3%N)) None
+          CharacterRange None))
+        (Some (Build_source_range
+          (Some (Build_physical_point 0 1%N 2%N 3%N))
+          (Some (Build_physical_point 0 4%N 5%N 6%N)) TokenRange
+          (Some (Build_physical_point 0 1%N 2%N 3%N,
+                 Build_physical_point 0 4%N 5%N 6%N))))
+    ; Build_macro_frame (Some "INLINE"%pstring) MacroBody
+        (Some (Build_source_range
+          (Some (Build_physical_point 0 1%N 2%N 3%N))
+          (Some (Build_physical_point 0 4%N 5%N 6%N)) CharacterRange
+          (Some (Build_physical_point 0 7%N 8%N 9%N,
+                 Build_physical_point 0 10%N 11%N 12%N)))) None
+    ] (Some (Build_physical_point 0 10%N 11%N 12%N)) (Some 1) [1].
+
+Definition rich_reference_origin : source_origin :=
+  test_origin ImplicitOrigin None [].
+
+Definition indexed_leaf_map
+    (tables : Encoded.indexed_provenance) (ids : list origin_id)
+    : source_map := {|
+  files := [];
+  origin_data := IndexedOrigins tables;
+  declarations := {|
+    symbol_locations := <[shared_root_name := leaf ids]> ∅;
+    type_locations := ∅;
+    msymbol_locations := ∅;
+    mtype_locations := ∅
+  |}
+|}.
+
+Example indexed_lookup_decodes_every_nested_field :
+  lookup (indexed_leaf_map rich_indexed_provenance [0])
+    (DRSymbol shared_root_name) [] = inr [rich_origin].
+Proof. vm_compute. reflexivity. Qed.
+
+Definition rich_expanded_map : source_map := {|
+  files := [];
+  origin_data := ExpandedOrigins [rich_origin; rich_reference_origin];
+  declarations :=
+    (indexed_leaf_map rich_indexed_provenance [0]).(declarations)
+|}.
+
+Example indexed_rich_lookup_matches_expanded_map :
+  lookup (indexed_leaf_map rich_indexed_provenance [0])
+    (DRSymbol shared_root_name) [] =
+  lookup rich_expanded_map (DRSymbol shared_root_name) [].
+Proof. vm_compute. reflexivity. Qed.
+
+Example indexed_diagnostic_materialization_matches_lookup_value :
+  Internal.materialize_origins (IndexedOrigins rich_indexed_provenance) =
+    inr [rich_origin; rich_reference_origin].
+Proof. vm_compute. reflexivity. Qed.
+
+Definition provenance_with_origins
+    (tables : Encoded.indexed_provenance)
+    (encoded_origins : list Encoded.encoded_origin)
+    : Encoded.indexed_provenance :=
+  Encoded.Build_indexed_provenance
+    tables.(Encoded.presumed_filename_table)
+    tables.(Encoded.physical_point_table)
+    tables.(Encoded.presumed_point_table)
+    tables.(Encoded.range_table)
+    tables.(Encoded.macro_frame_table)
+    (indexed_table_of_list Encoded.default_encoded_origin encoded_origins).
+
+Definition malformed_range_origin : Encoded.encoded_origin :=
+  Encoded.Build_encoded_origin ExplicitOrigin (Some 99%uint63) None
+    None None [] None None [].
+
+Definition malformed_anchor_origin : Encoded.encoded_origin :=
+  Encoded.Build_encoded_origin ExplicitOrigin (Some 99%uint63) None
+    None None [] None (Some 9) [].
+
+Definition malformed_derived_origin : Encoded.encoded_origin :=
+  Encoded.Build_encoded_origin ExplicitOrigin None None
+    None None [] None None [8; 7].
+
+Example indexed_lookup_reports_private_range_corruption :
+  lookup (indexed_leaf_map
+      (provenance_with_origins rich_indexed_provenance
+        [malformed_range_origin]) [0])
+    (DRSymbol shared_root_name) [] =
+  inl (MalformedProvenance (DRSymbol shared_root_name) [] 0
+    (Encoded.MissingTableEntry Encoded.RangeTable 99%uint63)).
+Proof. vm_compute. reflexivity. Qed.
+
+Example indexed_lookup_checks_anchor_before_nested_content :
+  lookup (indexed_leaf_map
+      (provenance_with_origins rich_indexed_provenance
+        [malformed_anchor_origin]) [0])
+    (DRSymbol shared_root_name) [] =
+  inl (OriginIdOutOfBounds (DRSymbol shared_root_name) [] 9).
+Proof. vm_compute. reflexivity. Qed.
+
+Example indexed_lookup_reports_first_invalid_derivation :
+  lookup (indexed_leaf_map
+      (provenance_with_origins rich_indexed_provenance
+        [malformed_derived_origin]) [0])
+    (DRSymbol shared_root_name) [] =
+  inl (OriginIdOutOfBounds (DRSymbol shared_root_name) [] 8).
+Proof. vm_compute. reflexivity. Qed.
+
+Definition unreachable_malformed_provenance : Encoded.indexed_provenance :=
+  provenance_with_origins rich_indexed_provenance
+    [rich_encoded_origin; malformed_range_origin].
+
+Example indexed_lookup_does_not_decode_unreachable_rows :
+  lookup (indexed_leaf_map unreachable_malformed_provenance [0])
+    (DRSymbol shared_root_name) [] = inr [rich_origin].
+Proof. vm_compute. reflexivity. Qed.
+
+Example indexed_lookup_decodes_only_until_first_failure :
+  lookup (indexed_leaf_map unreachable_malformed_provenance [1; 0])
+    (DRSymbol shared_root_name) [] =
+  inl (MalformedProvenance (DRSymbol shared_root_name) [] 1
+    (Encoded.MissingTableEntry Encoded.RangeTable 99%uint63)).
+Proof. vm_compute. reflexivity. Qed.
+
+Definition provenance_with_origin_table
+    (tables : Encoded.indexed_provenance)
+    (encoded_origins : Encoded.indexed_table Encoded.encoded_origin)
+    : Encoded.indexed_provenance :=
+  Encoded.Build_indexed_provenance
+    tables.(Encoded.presumed_filename_table)
+    tables.(Encoded.physical_point_table)
+    tables.(Encoded.presumed_point_table)
+    tables.(Encoded.range_table)
+    tables.(Encoded.macro_frame_table) encoded_origins.
+
+Definition missing_outer_origin_table
+    : Encoded.indexed_table Encoded.encoded_origin :=
+  Encoded.Build_indexed_table 1%uint63
+    (PArray.of_list
+      (PArray.of_list Encoded.default_encoded_origin []) []).
+
+Definition missing_inner_origin_table
+    : Encoded.indexed_table Encoded.encoded_origin :=
+  Encoded.Build_indexed_table 1%uint63
+    (PArray.of_list (PArray.of_list Encoded.default_encoded_origin [])
+      [PArray.of_list Encoded.default_encoded_origin []]).
+
+Example indexed_lookup_distinguishes_missing_outer_storage :
+  lookup (indexed_leaf_map
+      (provenance_with_origin_table rich_indexed_provenance
+        missing_outer_origin_table) [0])
+    (DRSymbol shared_root_name) [] =
+  inl (MalformedProvenance (DRSymbol shared_root_name) [] 0
+    (Encoded.MissingTableEntry Encoded.OriginTable 0%uint63)).
+Proof. vm_compute. reflexivity. Qed.
+
+Example indexed_lookup_distinguishes_missing_inner_storage :
+  lookup (indexed_leaf_map
+      (provenance_with_origin_table rich_indexed_provenance
+        missing_inner_origin_table) [0])
+    (DRSymbol shared_root_name) [] =
+  inl (MalformedProvenance (DRSymbol shared_root_name) [] 0
+    (Encoded.MissingTableEntry Encoded.OriginTable 0%uint63)).
+Proof. vm_compute. reflexivity. Qed.
+
+Definition storage_missing_anchor_origin : Encoded.encoded_origin :=
+  Encoded.Build_encoded_origin InheritedOrigin
+    None None None None [] None (Some 1) [].
+
+Definition storage_missing_derived_origin : Encoded.encoded_origin :=
+  Encoded.Build_encoded_origin InheritedOrigin
+    None None None None [] None None [1].
+
+Definition short_two_origin_table
+    (first : Encoded.encoded_origin)
+    : Encoded.indexed_table Encoded.encoded_origin :=
+  Encoded.Build_indexed_table 2%uint63
+    (PArray.of_list (PArray.of_list Encoded.default_encoded_origin [])
+      [PArray.of_list Encoded.default_encoded_origin [first]]).
+
+Example indexed_lookup_distinguishes_missing_anchor_storage :
+  lookup (indexed_leaf_map
+      (provenance_with_origin_table rich_indexed_provenance
+        (short_two_origin_table storage_missing_anchor_origin)) [0])
+    (DRSymbol shared_root_name) [] =
+  inl (MalformedProvenance (DRSymbol shared_root_name) [] 0
+    (Encoded.MissingTableEntry Encoded.OriginTable 1%uint63)).
+Proof. vm_compute. reflexivity. Qed.
+
+Example indexed_lookup_distinguishes_missing_derivation_storage :
+  lookup (indexed_leaf_map
+      (provenance_with_origin_table rich_indexed_provenance
+        (short_two_origin_table storage_missing_derived_origin)) [0])
+    (DRSymbol shared_root_name) [] =
+  inl (MalformedProvenance (DRSymbol shared_root_name) [] 0
+    (Encoded.MissingTableEntry Encoded.OriginTable 1%uint63)).
+Proof. vm_compute. reflexivity. Qed.
+
+Definition boundary_chunk0 : PArray.array nat :=
+  PArray.set (PArray.make 4096%uint63 0) 4095%uint63 7.
+
+Definition boundary_table : Encoded.indexed_table nat :=
+  Encoded.Build_indexed_table 4097%uint63
+    (PArray.of_list (PArray.of_list 0 [])
+      [boundary_chunk0; PArray.of_list 0 [8]]).
+
+Example indexed_table_chunk_boundaries :
+  ( Encoded.table_get boundary_table 4095%uint63
+  , Encoded.table_get boundary_table 4096%uint63
+  , Encoded.table_get boundary_table 4097%uint63 ) =
+  (Some 7, Some 8, None).
+Proof. vm_compute. reflexivity. Qed.
+
+Example indexed_empty_table_is_checked :
+  Encoded.table_get (indexed_table_of_list 0 []) 0%uint63 = None.
+Proof. vm_compute. reflexivity. Qed.
+
 Definition int_type : type := "int"%cpp_type.
 Definition bool_type : type := "bool"%cpp_type.
 
 Definition test_obj_value : ObjValue := Ovar int_type global_init.NoInit.
+
+Definition tactic_constructed_indexed_map : source_map.
+Proof.
+  Construction.build_indexed_source_map_or_fail ([] : list source_file)
+    unreachable_malformed_provenance
+    [Construction.LESymbol shared_root_name test_obj_value (leaf [0])].
+Defined.
+
+Example indexed_construction_does_not_decode_provenance :
+  lookup tactic_constructed_indexed_map (DRSymbol shared_root_name) [] =
+    inr [rich_origin].
+Proof. vm_compute. reflexivity. Qed.
 
 Example direct_obj_value_insertion_equivalence :
   translation_unit.list_decls
